fixcode.pl
@@ -39,6 +39,7 @@ import qualified Hask.Utils
 
     s/\(Prelude\.map  \( rs\)\)/rs/;
     s/\(Prelude\.map \)/(Prelude.map Prelude.id)/;
+    s/^   vars = IntMap.coq_IntMap_map $/   vars = Prelude.id /;
     s/mapLeft  /mapLeft Prelude.id /g;
     s/\(Data\.IntMap\.map  ranges\)/ranges/;
 
